src/tls/Old.HKDF.fst
@@ -1,10 +1,8 @@
-(**
-TLS 1.3 HKDF extract and expand constructions, parametrized by their hash algorithm
-*)
-module HKDF
-module HS = FStar.HyperStack //Added automatically
+module Old.HKDF
 
 open FStar.Bytes
+open FStar.HyperStack.ST
+
 open TLSConstants
 open Hashing.Spec
 
@@ -28,15 +26,32 @@ HKDF-Extract(salt, IKM) -> PRK
    PRK = HMAC-Hash(salt, IKM)
 *)
 
-val extract: 
-  #ha:hash_alg -> salt:hkey ha -> 
-  ikm:bytes -> 
-  ST (hkey ha)
+val hkdf_extract: ha:hash_alg -> salt:hkey ha -> ikm:bytes -> ST (tag ha)
   (requires (fun h0 -> True))
   (ensures (fun h0 t h1 -> FStar.HyperStack.modifies Set.empty h0 h1))
 
-let extract #ha salt ikm = HMAC.hmac ha salt ikm
+let hkdf_extract ha salt ikm = HMAC.hmac ha salt ikm
 
+private val hkdf_expand_int: ha:hash_alg
+  -> prk: hkey ha //was: bytes{tagLen ha <= length prk}
+  -> info:bytes
+  -> len:nat{len <= op_Multiply 255 (UInt32.v (tagLen ha))}
+  -> count:nat{count < 256 }
+  -> curr:nat{curr = op_Multiply count (UInt32.v (tagLen ha))}
+  -> prev:bytes
+  -> ST (b:bytes{len - curr <= length b}) (decreases (max 0 (len - curr)))
+  (requires (fun h0 -> True))
+  (ensures (fun h0 t h1 -> FStar.HyperStack.modifies Set.empty h0 h1))
+
+private let rec hkdf_expand_int ha prk info len count curr prev =
+  if curr < len && count + 1 < 256 then
+    let count = count + 1 in
+    let curr = curr + (UInt32.v (tagLen ha)) in
+    lemma_repr_bytes_values count;
+    let prev = HMAC.hmac ha prk (prev @| info @| bytes_of_int 1 count) in
+    let next = hkdf_expand_int ha prk info len count curr prev in
+    prev @| next
+  else empty_bytes
 
 (*-------------------------------------------------------------------*)
 (*
@@ -65,48 +80,15 @@ HKDF-Expand(PRK, info, L) -> OKM
    ...
 *)
 
-/// Generates enough bytes by concatenating HMAC blocks;
-/// no truncation yet.
-///
-/// Simple reduction to fixed-length PRF: if (info: bytes) is fresh,
-/// then the successive HMAC inputs are also fresh (by case on the
-/// *last* byte of the concatenated input of HMAC, separating the
-/// domain of the PRF into first blocks and others). On the other
-/// hand, the truncation length is not explicitly encoded here.
-/// 
-private val expand_int: 
-  #ha:hash_alg -> prk: hkey ha ->
-  info:bytes ->
-  len:nat{len <= op_Multiply 255 (tagLen ha)} ->
-  count:nat{count < 256 } ->
-  curr:nat{curr = op_Multiply count (tagLen ha)} ->
-  previous:bytes {length previous = (if count = 0 then 0 else tagLen ha)} -> 
-  ST (b:bytes{len - curr <= length b}) (decreases (max 0 (len - curr)))
+val hkdf_expand: ha:hash_alg
+  -> prk: hkey ha
+  -> info: bytes
+  -> len: nat{len <= op_Multiply 255 (UInt32.v (tagLen ha))}
+  -> ST (lbytes len)
   (requires (fun h0 -> True))
   (ensures (fun h0 t h1 -> FStar.HyperStack.modifies Set.empty h0 h1))
 
-#set-options "--z3rlimit 50"
-let rec expand_int #ha prk info len count curr previous =
-  if curr < len && count + 1 < 256 then
-    let count = count + 1 in
-    let curr = curr + tagLen ha in
-    lemma_repr_bytes_values count;
-    let block = HMAC.hmac ha prk (previous @| info @| bytes_of_int 1 count) in
-    let next = expand_int prk info len count curr block in
-    block @| next
-  else empty_bytes
-#reset-options
-
-/// Final truncation, possibly chopping of the end of the last block. 
-val expand: 
-  #ha:hash_alg -> prk: hkey ha ->
-  info: bytes -> 
-  len: nat{len <= op_Multiply 255 (tagLen ha)} ->
-  ST (lbytes len)
-  (requires (fun h0 -> True))
-  (ensures (fun h0 t h1 -> FStar.HyperStack.modifies Set.empty h0 h1))
-
-let expand #ha prk info len =
+let hkdf_expand ha prk info len =
   lemma_repr_bytes_values len;
   let raw = hkdf_expand_int ha prk info len 0 0 empty_bytes in
   fst(split_ raw len)  // possibly chopping off the end of the last hash
@@ -137,7 +119,7 @@ val hkdf_expand_label: ha: hash_alg
   -> prk: hkey ha
   -> label: string{length (bytes_of_string label) < 256 - 9}
   -> hv: bytes{length hv < 256}
-  -> len: nat{len <= op_Multiply 255 (tagLen ha)}
+  -> len: nat{len <= op_Multiply 255 (UInt32.v (tagLen ha))}
   -> ST (lbytes len)
   (requires (fun h0 -> True))
   (ensures (fun h0 t h1 -> FStar.HyperStack.modifies Set.empty h0 h1))
@@ -147,9 +129,12 @@ let hkdf_expand_label ha prk label hv len =
   lemma_repr_bytes_values len;
   lemma_repr_bytes_values (length label_bytes);
   lemma_repr_bytes_values (length hv);
-  bytes_of_int 2 len @|
-  vlbytes 1 label_bytes @|
-  vlbytes 1 hv 
+  let info = bytes_of_int 2 len @|
+	     Parse.vlbytes 1 label_bytes @|
+	     Parse.vlbytes 1 hv in
+  hkdf_expand ha prk info len
+
+
 
 (*-------------------------------------------------------------------*)
 (*
@@ -157,30 +142,24 @@ let hkdf_expand_label ha prk label hv len =
     HKDF-Expand-Label(Secret, Label,
        Transcript-Hash(Messages), Hash.length)
 *)
-/// renamed to expand_secret for uniformity
 
-val expand_secret:
-  #ha:hash_alg ->
+val derive_secret:
+  ha:hash_alg ->
   secret: hkey ha ->
   label: string{length (bytes_of_string label) < 256-6} ->
   hs_hash: bytes{length hs_hash < 256} ->
-  ST (hkey ha)
+  ST (lbytes (UInt32.v (Hashing.Spec.tagLen ha)))
   (requires fun h -> True)
   (ensures fun h0 _ h1 -> modifies_none h0 h1)
 
-
-// cwinter: verify
-// let expand_secret #ha prk label hv =
-//   expand_label prk label hv (Hashing.Spec.tagLen ha)
-  
 let derive_secret ha secret label hashed_log =
   let lbl = tls13_prefix @| bytes_of_string label in
   cut(length lbl < 256);
-  lemma_repr_bytes_values (Hashing.Spec.tagLen ha);
+  lemma_repr_bytes_values (UInt32.v (Hashing.Spec.tagLen ha));
   lemma_repr_bytes_values (length lbl);
   lemma_repr_bytes_values (length hashed_log);
   let info =
-    bytes_of_int 2 (Hashing.Spec.tagLen ha) @|
-    vlbytes 1 lbl @|
-    vlbytes 1 hashed_log in
-  hkdf_expand ha secret info (Hashing.Spec.tagLen ha)
+    bytes_of_int 2 (UInt32.v (Hashing.Spec.tagLen ha)) @|
+    Parse.vlbytes 1 lbl @|
+    Parse.vlbytes 1 hashed_log in
+  hkdf_expand ha secret info (UInt32.v (Hashing.Spec.tagLen ha))
